src/SoftBound/sb_ds_metadata.v
@@ -1,0 +1,1076 @@
+Add LoadPath "../ssa/ott".
+Add LoadPath "../ssa/monads".
+Add LoadPath "../ssa".
+Add LoadPath "../ssa/compcert".
+Add LoadPath "../../../theory/metatheory_8.3".
+Add LoadPath "../TV".
+Require Import ssa_def.
+Require Import ssa_lib.
+Require Import List.
+Require Import Arith.
+Require Import tactics.
+Require Import monad.
+Require Import trace.
+Require Import Metatheory.
+Require Import genericvalues.
+Require Import alist.
+Require Import Values.
+Require Import Memory.
+Require Import Integers.
+Require Import Coqlib.
+Require Import targetdata.
+Require Import Maps.
+Require Import Lattice.
+Require Import Iteration.
+Require Import Kildall.
+Require Import ssa_static.
+Require Import ssa_props.
+Require Import ssa_analysis.
+Require Import ssa_wf.
+Require Import ssa_dynamic.
+Require Import sb_ds_def.
+Require Import sbop_dsop.
+Require Import Znumtheory.
+
+Ltac zauto := auto with zarith.
+
+Tactic Notation "bdestruct" ident(H) "as" ident(J1) ident(J2) :=
+     apply andb_true_iff in H; destruct H as [J1 J2].
+
+Tactic Notation "bdestruct3" ident(H) "as" ident(J1) ident(J2) ident(J3) :=
+     bdestruct H as H J3;
+     bdestruct H as J1 J2.
+
+Tactic Notation "bdestruct4" ident(H) "as" ident(J1) ident(J2) ident(J3) ident(J4) :=
+     bdestruct3 H as H J3 J4;
+     bdestruct H as J1 J2.
+
+Tactic Notation "bdestruct5" ident(H) "as" ident(J1) ident(J2) ident(J3) ident(J4) ident(J5) :=
+     bdestruct4 H as H J3 J4 J5;
+     bdestruct H as J1 J2.
+
+Ltac bdestructn H Js :=
+  match Js with
+  | nil => idtac
+  | ?J::nil => rename H into J
+  | ?J::?Js' => apply andb_true_iff in H; destruct H as [H J]; bdestructn H Js
+  end.
+
+Ltac bsplit :=
+  eapply andb_true_iff; split.
+
+Ltac repeat_bsplit :=
+  repeat (bsplit; auto using eq_sumbool2bool_true).
+
+Ltac zeauto := eauto with zarith.
+
+(*****************************************)
+(* wf_data *)
+
+Export LLVMgv.
+Export SBopsem.
+
+Definition wf_data (TD:TargetData) (M:mem) (gvb gve:GenericValue) : Prop :=
+  match (GV2ptr TD (getPointerSize TD) gvb,
+         GV2ptr TD (getPointerSize TD) gve) with
+  | (Some (Values.Vptr bb bofs), Some (Values.Vptr eb eofs)) =>
+      if zeq bb eb then
+        bb < Mem.nextblock M /\
+        (blk_temporal_safe M bb ->
+         Mem.range_perm M bb (Int.signed 31 bofs) (Int.signed 31 eofs) Writable)
+      else False
+  | _ => False
+  end.
+
+Definition wf_rmetadata (TD:TargetData) (M:mem) (rm:rmetadata) : Prop :=
+  forall (i:id) (gvb gve:GenericValue),
+    lookupAL _ rm i = Some (mkMD gvb gve) -> wf_data TD M gvb gve.
+
+Definition wf_mmetadata (TD:TargetData) (M:mem) (MM:mmetadata) : Prop :=
+  forall (b:Values.block) (ofs:int32) (gvb gve:GenericValue),
+    MM b ofs = Some (mkMD gvb gve) -> wf_data TD M gvb gve.
+
+Definition wf_metadata (TD:TargetData) (M:mem) (rm:rmetadata) (MM:mmetadata) 
+    : Prop :=
+  wf_rmetadata TD M rm /\ wf_mmetadata TD M MM.
+
+Lemma range_perm_alloc_other:
+  forall m1 lo hi m2 b, Mem.alloc m1 lo hi = (m2, b) ->
+  forall b' lo' hi' p,
+  Mem.range_perm m1 b' lo' hi' p ->
+  Mem.range_perm m2 b' lo' hi' p.
+Proof.
+  intros.
+  unfold Mem.range_perm in *.
+  intros ofs J.
+  apply H0 in J.
+  eapply Mem.perm_alloc_1; eauto.
+Qed.
+
+Lemma store_range_perm_1:
+  forall chunk m1 b ofs v m2, Mem.store chunk m1 b ofs v = Some m2 ->
+  forall b' lo' hi' p,
+  Mem.range_perm m1 b' lo' hi' p -> Mem.range_perm m2 b' lo' hi' p.
+Proof.
+  intros.
+  unfold Mem.range_perm in *.
+  intros ofs0 J.
+  apply H0 in J.
+  eapply Mem.perm_store_1; eauto.
+Qed.
+
+Lemma GV2ptr_base2GV : forall TD mb,
+  GV2ptr TD (getPointerSize TD) (base2GV TD mb) = 
+    Some (Values.Vptr mb (Int.repr 31 0)).
+Proof.
+  intros TD mb.
+  unfold GV2ptr. unfold base2GV. unfold blk2GV. unfold ptr2GV. unfold val2GV.
+  auto.
+Qed.
+
+Lemma GV2ptr_bound2GV : forall TD mb tsz n,
+  GV2ptr TD (getPointerSize TD) (bound2GV TD mb tsz n) = 
+    Some (Values.Vptr mb (Int.repr 31 ((Size.to_Z tsz)*n))).
+Proof.
+  intros TD mb tsz n.
+  unfold GV2ptr. unfold bound2GV. unfold ptr2GV. unfold val2GV.
+  auto.
+Qed.
+
+Lemma wf_mmetadata__wf_data : forall Mem0 TD MM b0 ofs gvb gve,
+  wf_mmetadata TD Mem0 MM ->
+  MM b0 ofs = Some (mkMD gvb gve) ->
+  wf_data TD Mem0 gvb gve.
+Proof.
+  intros Mem0 TD MM b0 ofs gvb gve Hwfm J.
+  apply Hwfm in J; clear Hwfm.
+  unfold wf_data in *.
+  destruct (GV2ptr TD (getPointerSize TD) gvb); auto.
+Qed.
+
+Lemma blk_temporal_safe_store_2 : forall m Mem0 b ofs0 v0 Mem' b0,
+  Mem.store m Mem0 b ofs0 v0 = Some Mem' ->
+  blk_temporal_safe Mem' b0 ->
+  blk_temporal_safe Mem0 b0. 
+Proof.
+  intros m Mem0 b ofs0 v0 Mem' b0 Hstore H.
+  unfold blk_temporal_safe in *.
+  assert (J:=Hstore).
+  apply Mem.bounds_store with (b':=b0) in J.
+  rewrite <- J.
+  destruct (Mem.bounds Mem' b0).
+  eapply Mem.perm_store_2 in H; eauto.  
+Qed.
+
+Lemma wf_data__store__wf_data : forall m Mem0 b ofs0 v0 Mem' TD gvb gve,
+  Mem.store m Mem0 b ofs0 v0 = Some Mem' ->
+  wf_data TD Mem0 gvb gve ->
+  wf_data TD Mem' gvb gve.
+Proof.
+  intros m Mem0 b ofs0 v0 Mem' TD gvb gve H1 J.
+  unfold wf_data in *.
+  destruct (GV2ptr TD (getPointerSize TD) gvb); auto.
+  destruct v; auto.
+  destruct (GV2ptr TD (getPointerSize TD) gve); auto.
+  destruct v; auto.
+  destruct (zeq b0 b1); auto.
+    destruct J as [J1 J2].
+    split.
+      apply Mem.nextblock_store in H1.
+      rewrite H1. auto.
+
+      intro H.
+      eapply blk_temporal_safe_store_2 in H; eauto.
+      apply J2 in H.
+      eauto using store_range_perm_1.
+Qed.
+
+Lemma wf_mmetadata__store__wf_data : forall m Mem0 b ofs0 v0 Mem' TD MM b0 ofs 
+    gvb gve,
+  Mem.store m Mem0 b ofs0 v0 = Some Mem' ->
+  wf_mmetadata TD Mem0 MM ->
+  MM b0 ofs = Some (mkMD gvb gve) ->
+  wf_data TD Mem' gvb gve.
+Proof.
+  intros m Mem0 b ofs0 v0 Mem' TD MM b0 ofs gvb gve H1 Hwfm J.
+  apply wf_mmetadata__wf_data with (Mem0:=Mem0)(TD:=TD) in J; eauto.
+  eapply wf_data__store__wf_data; eauto.
+Qed.
+
+Definition wf_global_ptr S TD Mem0 gl : Prop :=
+  forall id0 gv0 typ0, lookupAL GenericValue gl id0 = Some gv0 ->
+  wf_const S TD (const_gid typ0 id0) (typ_pointer typ0) ->
+  exists b, exists sz,
+    GV2ptr TD (getPointerSize TD) gv0 = Some (Values.Vptr b ((Int.zero 31))) /\
+    b < Mem.nextblock Mem0 /\
+    getTypeAllocSize TD typ0 = Some sz /\
+    Mem.bounds Mem0 b = (0, Z_of_nat sz) /\
+    (blk_temporal_safe Mem0 b -> Mem.range_perm Mem0 b 0 (Z_of_nat sz) Writable).
+
+Lemma get_const_metadata_gid__wf_data : forall S TD Mem0 gl t i0 gvb gve,
+  wf_global_ptr S TD Mem0 gl ->
+  wf_const S TD (const_gid t i0) (typ_pointer t) ->
+  const2GV TD Mem0 gl (const_gid t i0) = ret gvb ->
+  const2GV TD Mem0 gl
+         (const_gep false (const_gid t i0)
+            (Cons_list_const (const_int Size.ThirtyTwo 1) Nil_list_const)) =
+       ret gve ->
+  wf_data TD Mem0 gvb gve.
+Proof.
+  intros S TD Mem0 gl t i0 gvb gve Hwfg Hwfc H2 H3.
+  unfold const2GV in H3.
+  remember (_const2GV TD Mem0 gl
+           (const_gep false (const_gid t i0)
+              (Cons_list_const (const_int Size.ThirtyTwo 1) Nil_list_const))) 
+    as R0.
+  destruct R0; try solve [inversion H3].
+  destruct p. inv H3.
+  unfold const2GV in H2.
+  remember (_const2GV TD Mem0 gl (const_gid t i0)) as R1.
+  destruct R1; try solve [inversion H2].
+  destruct p. inv H2.
+  unfold _const2GV in *.
+  remember (lookupAL GenericValue gl i0) as R'.
+  destruct R'; try solve [inversion HeqR0].
+  inv HeqR1.
+  remember (getConstGEPTyp
+              (Cons_list_const (const_int Size.ThirtyTwo 1) Nil_list_const)
+              (typ_pointer t)) as R1.
+  destruct R1; try solve [inversion HeqR0].
+  symmetry in HeqR'.
+  assert (exists b, exists sz,
+    GV2ptr TD (getPointerSize TD) g = Some (Values.Vptr b ((Int.zero 31))) /\
+    b < Mem.nextblock Mem0 /\
+    getTypeAllocSize TD t = Some sz /\
+    Mem.bounds Mem0 b = (0, Z_of_nat sz) /\
+    (blk_temporal_safe Mem0 b -> Mem.range_perm Mem0 b 0 (Z_of_nat sz) Writable))
+    as J.
+    eapply Hwfg; eauto.
+  destruct J as [b [sz [J1 [J2 [J3 [J4 J5]]]]]].
+  rewrite J1 in HeqR0.
+  simpl in HeqR0.
+  unfold mgetoffset in HeqR0.
+  destruct TD.
+  assert (exists ut2, typ2utyp l1 (typ_array 0%nat t) = 
+    Some (typ_array 0%nat ut2) /\
+    getTypeAllocSize (l0, l1) ut2 = getTypeAllocSize (l0, l1) t) as J.
+    unfold typ2utyp. simpl.
+    admit. (* wft *)
+  destruct J as [ut2 [J6 J7]].
+  rewrite J6 in HeqR0. simpl in HeqR0.
+  rewrite J7 in HeqR0. rewrite J3 in HeqR0. simpl in HeqR0.
+  inv HeqR0.
+  unfold wf_data. rewrite J1. simpl.
+  destruct (zeq b b); auto.
+    split; auto.
+    admit. (* int *)
+Qed.
+
+Lemma eq_gv_is_wf_data : forall TD Mem gv bb bofs,
+  bb < Mem.nextblock Mem ->
+  GV2ptr TD (getPointerSize TD) gv = Some (Values.Vptr bb bofs) ->
+  wf_data TD Mem gv gv.
+Proof.
+  intros TD Mem gv bb bofs H0 H.
+  unfold wf_data.
+  rewrite H.
+  destruct (zeq bb bb); auto.
+  split; auto.
+    intros Hwfb ofs J.
+    contradict J; zauto.
+Qed.
+
+Lemma nullptr_lt_nextblock : forall Mem0,
+  Mem.nullptr < Mem.nextblock Mem0.
+Proof.
+  intros.
+  assert (J:=@Mem.nextblock_pos Mem0).
+  unfold Mem.nullptr.
+  zauto.
+Qed.
+
+Lemma null_is_wf_data : forall TD Mem,
+  wf_data TD Mem null null.
+Proof.
+  intros TD Mem.
+  eapply eq_gv_is_wf_data with (bb:=Mem.nullptr).
+    apply nullptr_lt_nextblock.
+
+    unfold GV2ptr.
+    simpl. eauto.
+Qed.
+
+Lemma wf_rmetadata__get_const_metadata : forall S TD gl Mem0 rm c gvb gve c0 c1
+   ct ct',
+  wf_global_ptr S TD Mem0 gl ->
+  wf_const S TD c ct' ->
+  wf_rmetadata TD Mem0 rm ->
+  get_const_metadata c = Some (c0,c1,ct) ->
+  const2GV TD Mem0 gl c0 = Some gvb ->
+  const2GV TD Mem0 gl c1 = Some gve ->
+  wf_data TD Mem0 gvb gve.
+Proof.
+  induction c; intros gvb gve cc0 cc1 ct ct' Hwfg Hwfc Hwfr H1 H2 H3; 
+    try solve [inversion H1].
+
+  inv Hwfc.
+  destruct t; inv H1; 
+    try solve [ 
+      eapply get_const_metadata_gid__wf_data; eauto using wf_const_gid
+    ].
+
+    unfold const2GV in H2, H3.
+    remember (_const2GV TD Mem0 gl (const_gid (typ_function t l0 v) i0)) as R.
+    destruct R; try solve [inversion H2 | inversion H3].
+    destruct p. inv H2. inv H3.
+    unfold GV2ptr.
+    unfold _const2GV in HeqR.
+    remember (lookupAL GenericValue gl i0) as R1.
+    destruct R1; inv HeqR.
+    assert (exists b, exists sz,
+      GV2ptr TD (getPointerSize TD) g = Some (Values.Vptr b ((Int.zero 31))) /\
+      b < Mem.nextblock Mem0 /\
+      getTypeAllocSize TD (typ_function t l0 v) = Some sz /\
+      Mem.bounds Mem0 b = (0, Z_of_nat sz) /\
+      (blk_temporal_safe Mem0 b -> Mem.range_perm Mem0 b 0 (Z_of_nat sz) Writable))
+      as J.
+      eapply Hwfg; eauto using wf_const_gid.
+    destruct J as [b [sz [J1 [J2 [J3 [J4 J5]]]]]].
+    eapply eq_gv_is_wf_data; eauto.
+
+  simpl in H1.
+  destruct c; try solve [inversion H1].
+  destruct t; try solve [inversion H1].
+  inv Hwfc.
+  eapply IHc; eauto.
+     
+  inv Hwfc.
+  simpl in H1; eauto.
+Qed.
+
+Lemma wf_rmetadata__get_reg_metadata : forall S los nts Ps Mem0 rm gl vp gvb gve 
+    t f tp,
+  wf_global_ptr S (los, nts) Mem0 gl ->
+  wf_rmetadata (los, nts) Mem0 rm ->
+  wf_value S (module_intro los nts Ps) f vp tp ->
+  get_reg_metadata (los, nts) Mem0 gl rm vp = Some (mkMD gvb gve, t) ->
+  wf_data (los, nts) Mem0 gvb gve.
+Proof.
+  intros S los nts Ps Mem0 rm gl vp gvb gve t f tp Hwfg Hwfr Hwfv J.
+  unfold get_reg_metadata in J.
+  destruct vp.
+    remember (lookupAL metadata rm i0) as R.
+    destruct R; inv J.
+    symmetry in HeqR.
+    apply Hwfr in HeqR; auto.
+
+    remember (get_const_metadata c) as R.
+    destruct R as [[[bc ec] ct] |]; 
+      try solve [inversion J; subst; auto using null_is_wf_data].
+    remember (const2GV (los, nts) Mem0 gl bc) as R0.
+    remember (const2GV (los, nts) Mem0 gl ec) as R1.
+    destruct R0; try solve [inversion J]. 
+    simpl in J.
+    destruct R1; try solve [inversion J]. 
+    simpl in J.
+    inv J.
+    inv Hwfv.
+    eapply wf_rmetadata__get_const_metadata; eauto.
+Qed.
+
+Lemma wf_mmetadata__get_mem_metadata : forall TD Mem0 MM gvp gvb gve,
+  wf_mmetadata TD Mem0 MM ->
+  get_mem_metadata TD MM gvp = mkMD gvb gve ->
+  wf_data TD Mem0 gvb gve.
+Proof.
+  intros TD Mem0 MM gvp gvb gve Hwfm H4.
+  unfold get_mem_metadata in H4.
+  remember (GV2ptr TD (getPointerSize TD) gvp) as R.
+  destruct R; try solve [inversion H4; subst; auto using null_is_wf_data].
+  destruct v; try solve [inversion H4; subst; auto using null_is_wf_data].
+  remember (MM b i0) as R'.
+  destruct R'; inv H4; auto using null_is_wf_data.
+  symmetry in HeqR'.     
+  apply Hwfm in HeqR'; auto.
+Qed.
+
+Lemma blk_temporal_alloc_inv : forall Mem0 lo hi Mem' mb b0,
+  Mem.alloc Mem0 lo hi = (Mem', mb) ->
+  blk_temporal_safe Mem' b0 ->
+  (if Values.eq_block b0 mb then 
+    Mem.bounds Mem' b0 = (lo, hi)
+  else blk_temporal_safe Mem0 b0).
+Proof.
+  intros.
+  unfold blk_temporal_safe in *.
+  assert (Halloc := H).  
+  apply Mem.bounds_alloc with (b':=b0) in H.
+  destruct (Values.eq_block b0 mb); subst; auto.
+    rewrite <- H.
+    destruct (Mem.bounds Mem' b0).
+    apply Mem.perm_alloc_inv with (b':=b0)(ofs:=z)(p:=Nonempty) in Halloc; auto.
+    destruct (zeq b0 mb); auto.
+      subst. contradict n; auto.
+Qed.
+
+Lemma assert_mptr_dec : forall TD t ptr md,
+  assert_mptr TD t ptr md \/ ~ assert_mptr TD t ptr md.
+Proof.
+  intros.
+  unfold is_true. 
+  destruct (assert_mptr TD t ptr md); auto.
+Qed.
+
+Lemma typ2memory_chunk__le__getTypeAllocSize : forall t c s TD,
+  typ2memory_chunk t = Some c ->
+  Some s = getTypeAllocSize TD t ->
+  size_chunk c <= Size.to_Z s.
+Proof.
+  intros t c s TD H1 H2.
+  unfold getTypeAllocSize, getTypeStoreSize, getTypeSizeInBits, 
+         getTypeSizeInBits_and_Alignment in H2.
+  destruct TD.
+  destruct t; inv H1; inv H2;
+    simpl; unfold bytesize_chunk, Size.to_nat, RoundUpAlignment, Size.to_Z, ndiv.
+    assert (Z_of_nat (s0 + 7) / Z_of_nat 8 >= 0) as J.
+      assert (J1:=@Z_of_S_gt_O (s0 + 6)).
+      assert (S (s0 + 6) = (s0 + 7)%nat) as EQ. auto.
+      rewrite EQ in J1.        
+      assert (J2:=@O_lt_Z_of_S 7).
+      assert (0 <= Z_of_nat (s0 + 7) / Z_of_nat 8) as J3.
+        apply Z_div_pos; auto with zarith.
+       zauto.
+    assert (two_power_nat (getIntAlignmentInfo l0 s0 true) >= 0 ) as J2.
+      admit. (* zarith *)
+    rewrite nat_of_Z_eq.
+      rewrite nat_of_Z_eq; auto.
+        admit. (* zarith *)
+      rewrite nat_of_Z_eq; auto.
+        admit. (* zarith *)
+
+    destruct f; inv H0; inv H1; simpl; unfold RoundUpAlignment, ndiv.
+      assert (Z_of_nat 39 / Z_of_nat 8 = 4) as EQ.
+        simpl. admit. (* zarith *) 
+      rewrite EQ.
+      rewrite nat_of_Z_eq.
+        rewrite nat_of_Z_eq.
+(*
+Z_mod_lt
+Z_div_plus_full
+Z_div_mod_eq_full
+*)
+          admit. (* zarith *) 
+          zauto. (* zarith *) 
+        rewrite nat_of_Z_eq.
+          admit. (* zarith *) 
+          zauto. (* zarith *) 
+
+      assert (Z_of_nat 71 / Z_of_nat 8 = 8) as EQ.
+        simpl. admit. (* zarith *) 
+      rewrite EQ.
+      rewrite nat_of_Z_eq.
+        rewrite nat_of_Z_eq.
+          admit. (* zarith *) 
+          zauto. (* zarith *) 
+        rewrite nat_of_Z_eq.
+          admit. (* zarith *) 
+          zauto. (* zarith *) 
+
+    unfold getPointerSizeInBits.
+    unfold getPointerSize0.
+    admit. (* assume getPointerSizeInBits = 32 *)
+Qed.
+
+Lemma assert_mptr__valid_access : forall S md los nts Ps Mem gl rm MM t g b ofs
+    c mt f v tv,
+  wf_metadata (los, nts) Mem rm MM ->
+  wf_global_ptr S (los, nts) Mem gl ->
+  wf_value S (module_intro los nts Ps) f v tv ->
+  Some (md,mt) = get_reg_metadata (los, nts) Mem gl rm v ->
+  assert_mptr (los, nts) t g md ->
+  GV2ptr (los, nts) (getPointerSize (los, nts)) g = ret Values.Vptr b ofs ->
+  typ2memory_chunk t = ret c ->
+  (align_chunk c | Int.signed 31 ofs) ->
+  blk_temporal_safe Mem b ->
+  Mem.valid_access Mem c b (Int.signed 31 ofs) Writable.
+Proof.
+  intros S md los nts Ps Mem gl rm MM t g b ofs c mt f v tv Hwf Hwfg Hwfv Heqmd
+    J R3 R4 R5 Htmp.
+  unfold Mem.valid_access.
+  split; auto.
+    unfold assert_mptr in J.
+    rewrite R3 in J.
+    symmetry in Heqmd.  
+    destruct md.
+    destruct Hwf as [Hwfr Hwfm].
+    eapply wf_rmetadata__get_reg_metadata in Heqmd; eauto.
+    unfold wf_data in Heqmd.
+    unfold layouts, namedts in J.
+    destruct (GV2ptr (@pair (list layout) (list namedt) los nts)
+              (getPointerSize (@pair (list layout) (list namedt) los nts))
+              md_base0);
+      try solve [inversion Heqmd].
+    destruct v0; try solve [inversion Heqmd].
+    destruct (GV2ptr (@pair (list layout) (list namedt) los nts)
+              (getPointerSize (@pair (list layout) (list namedt) los nts))
+              md_bound0);
+      try solve [inversion Heqmd].
+    destruct v0; try solve [inversion Heqmd].
+    destruct (zeq b0 b1); subst; try solve [inversion Heqmd].
+    remember (getTypeAllocSize (@pair (list layout) (list namedt) los nts) t)
+      as R6.
+    destruct R6; try solve [inversion J].
+    simpl in J.
+    intros z Jz.
+    bdestruct4 J as J1 J4 J2 J3.
+    destruct (zeq b b1); subst; try solve [inversion J1].
+    apply Heqmd; auto.
+    clear - J2 J3 Jz HeqR6 R4.
+    assert (size_chunk c <= Size.to_Z s) as J4.
+      eapply typ2memory_chunk__le__getTypeAllocSize; eauto.
+    destruct (zle (Int.signed 31 i0) (Int.signed 31 ofs)); 
+      simpl in J2; inversion J2.
+    destruct (zle (Int.signed 31 ofs + Size.to_Z s) (Int.signed 31 i1)); 
+      simpl in J3; inversion J3.
+    zeauto.
+Qed.
+
+Lemma blk_temporal_safe_dec : forall M b,
+  {blk_temporal_safe M b} + {~ blk_temporal_safe M b}.
+Proof.
+  intros M b.
+  unfold blk_temporal_safe.
+  destruct (Mem.bounds M b).
+  apply Mem.perm_dec.
+Qed.
+
+Lemma valid_block_dec : forall M b,
+  {Mem.valid_block M b} + { ~ Mem.valid_block M b}.
+Proof.
+  intros M b.
+  unfold Mem.valid_block.
+  apply Z_lt_dec; auto.
+Qed.  
+
+Lemma free_preserves_wf_data : forall TD (Mem0 Mem' : mem) (b : Values.block)
+  (z z0 : Z) (HeqR : (z, z0) = Mem.bounds Mem0 b)
+  (H0 : Mem.free Mem0 b z z0 = ret Mem') (gvb gve : GenericValue)
+  (J : wf_data TD Mem0 gvb gve),
+  wf_data TD Mem' gvb gve.
+Proof.
+  intros.
+    unfold wf_data in *.
+    remember (GV2ptr TD (getPointerSize TD) gvb) as Rb.
+    destruct Rb; auto.
+    destruct v; auto.
+    remember (GV2ptr TD (getPointerSize TD) gve) as Re.
+    destruct Re; auto.
+    destruct v; auto.
+    destruct (zeq b0 b1); subst; auto. 
+    destruct J as [J1 J2].
+    split.
+      apply Mem.nextblock_free in H0.
+      rewrite H0. auto.
+
+      intro Hwfb.
+      unfold blk_temporal_safe in *.
+      erewrite Mem.bounds_free in Hwfb; eauto.
+      assert (Hfree:=H0).
+      destruct (Values.eq_block b b1); subst.
+        rewrite <- HeqR in Hwfb.
+        destruct (Z_lt_dec z z0).
+          apply Mem.perm_free_2 with (ofs:=z)(p:=Nonempty) in H0; 
+            zeauto.
+          contradict Hwfb; auto.
+
+          rewrite <- HeqR in J2.   
+          eapply Mem.perm_free_3 in Hwfb; eauto.
+          apply J2 in Hwfb. clear J2.
+          unfold Mem.range_perm in *.
+          intros ofs J. apply Hwfb in J.
+          apply Mem.perm_free_1 with (b:=b1)(ofs:=ofs)(p:=Writable) in H0; auto.
+            clear - n.
+            destruct (Z_lt_dec ofs z); auto.
+            destruct (Z_le_dec z0 ofs); auto.
+            assert (False) as H. zeauto. 
+            inversion H.
+
+       destruct (Mem.bounds Mem0 b1).
+       eapply Mem.perm_free_3 in Hwfb; eauto.
+       apply J2 in Hwfb. clear J2.
+       unfold Mem.range_perm in *.
+       intros ofs J. apply Hwfb in J.
+        apply Mem.perm_free_1 with (b:=b1)(ofs:=ofs)(p:=Writable) in H0;
+          zeauto.
+Qed.     
+
+Lemma free_preserves_wf_rmetadata : forall TD (Mem0 Mem' : mem) gv 
+  (H0 : free TD Mem0 gv = ret Mem') rm (Hwfr : wf_rmetadata TD Mem0 rm),
+  wf_rmetadata TD Mem' rm.
+Proof.
+  intros. 
+  unfold free in H0.
+  destruct (GV2ptr TD (getPointerSize TD) gv); try solve [inv H0].
+  destruct v; try solve [inv H0].
+  destruct (zeq (Int.signed 31 i0) 0); try solve [inv H0].
+  remember (Mem.bounds Mem0 b) as R.
+  destruct R as [l h].
+  intros i1 gvb gve J.
+  apply Hwfr in J.   
+  eapply free_preserves_wf_data; eauto.
+Qed.
+
+Lemma free_preserves_wf_mmetadata : forall TD (Mem0 Mem' : mem) gv
+  (H0 : free TD Mem0 gv = ret Mem') MM (Hwfm : wf_mmetadata TD Mem0 MM),
+  wf_mmetadata TD Mem' MM.
+Proof.
+  intros. 
+  unfold free in H0.
+  destruct (GV2ptr TD (getPointerSize TD) gv); try solve [inv H0].
+  destruct v; try solve [inv H0].
+  destruct (zeq (Int.signed 31 i0) 0); try solve [inv H0].
+  remember (Mem.bounds Mem0 b) as R.
+  destruct R as [l h].
+  intros b1 ofs gvb gve J.
+  assert (J':=@Hwfm b1 ofs gvb gve J).
+  eapply free_preserves_wf_data; eauto.
+Qed.
+
+Lemma free_allocas_preserves_wf_rmetadata : forall als TD M M' rm,
+  free_allocas TD M als = Some M' ->
+  wf_rmetadata TD M rm ->
+  wf_rmetadata TD M' rm.
+Proof.
+  induction als; simpl; intros TD M M' rm Hfree Hwfr.
+    inv Hfree. auto.
+
+    remember (free TD M (blk2GV TD a)) as R.
+    destruct R; inv Hfree.
+    eapply IHals; eauto.
+    eapply free_preserves_wf_rmetadata in Hwfr; eauto.
+Qed.
+
+Lemma free_allocas_preserves_wf_mmetadata : forall als TD M M' MM,
+  free_allocas TD M als = Some M' ->
+  wf_mmetadata TD M MM ->
+  wf_mmetadata TD M' MM.
+Proof.
+  induction als; simpl; intros TD M M' MM Hfree Hwfr.
+    inv Hfree. auto.
+
+    remember (free TD M (blk2GV TD a)) as R.
+    destruct R; inv Hfree.
+    eapply IHals; eauto.
+    eapply free_preserves_wf_mmetadata in Hwfr; eauto.
+Qed.
+
+Lemma alloc_preserves_wf_data : forall TD Mem0 sz Mem' mb
+  (H4 : Mem.alloc Mem0 0 sz = (Mem', mb))
+  (gvb : GenericValue)
+  (gve : GenericValue)
+  (J' : wf_data TD Mem0 gvb gve),
+  wf_data TD Mem' gvb gve.
+Proof.
+  intros.
+  unfold wf_data in *.
+  remember (GV2ptr TD (getPointerSize TD) gvb) as Rb.
+  destruct Rb; auto.
+  destruct v; auto.
+  remember (GV2ptr TD (getPointerSize TD) gve) as Re.
+  destruct Re; auto.
+  destruct v; auto.
+  destruct (zeq b b0); subst; auto. 
+  destruct J' as [J1' J2'].
+  split.
+    apply Mem.nextblock_alloc in H4.
+    rewrite H4. zauto.
+
+    intro Hwfb.
+    assert (Halloc := H4).
+    eapply blk_temporal_alloc_inv in H4; eauto.         
+    destruct (Values.eq_block b0 mb); subst.
+      apply Mem.alloc_result in Halloc.    
+      rewrite <- Halloc in J1'.
+      contradict J1'; zauto.
+      
+      apply J2' in H4.
+      eauto using range_perm_alloc_other.
+Qed.
+
+Lemma malloc_preserves_wf_rmetadata : forall
+  (TD : TargetData)
+  (rm : AssocList metadata)
+  (lc : GVMap)
+  (gl : GVMap)
+  (id0 : atom)
+  (t : typ)
+  (v : value)
+  (gn : GenericValue)
+  (align0 : align)
+  (Mem0 : mem)
+  (Mem' : mem)
+  (tsz : sz)
+  (mb : mblock)
+  (lc' : GVMap)
+  (rm' : rmetadata)
+  (n : Z)
+  (H : getTypeAllocSize TD t = ret tsz)
+  (H0 : getOperandValue TD Mem0 v lc gl = ret gn)
+  (H1 : malloc TD Mem0 tsz gn align0 = ret (Mem', mb))
+  (H2 : GV2int TD Size.ThirtyTwo gn = ret n)
+  (H3 : prop_reg_metadata lc rm id0 (blk2GV TD mb)
+         {| md_base := base2GV TD mb; md_bound := bound2GV TD mb tsz n |} =
+       (lc', rm'))
+  (Hwfr : wf_rmetadata TD Mem0 rm),
+  wf_rmetadata TD Mem' rm'.
+Proof.
+  intros.
+  invert_prop_reg_metadata. clear H3.
+  unfold malloc in H1.
+  rewrite H2 in H1.
+  remember (Mem.alloc Mem0 0 (Size.to_Z tsz * n)) as R.
+  inversion H1. clear H1. subst.
+  clear H2.
+  intros i0 gvb gve J.
+  destruct (@id_dec id0 i0); subst.
+  SCase "id0=i0".
+      rewrite lookupAL_updateAddAL_eq in J.
+      inversion J; subst. clear J.
+      unfold wf_data.
+      rewrite GV2ptr_base2GV. 
+      rewrite GV2ptr_bound2GV. 
+      destruct (zeq mb mb) as [J | J]; try solve [contradict J; auto].
+      split.
+        assert (H4':=H4).
+        apply Mem.alloc_result in H4.
+        apply Mem.nextblock_alloc in H4'.
+        rewrite H4. rewrite H4'. zauto.
+
+        intros Hwfb ofs J1. 
+        apply Mem.valid_access_alloc_same with (ofs:=ofs)(chunk:=AST.Mint 7) 
+          in H4.
+          destruct H4 as [J2 J3].
+          unfold Mem.range_perm in J2.
+          apply Mem.perm_implies with (p1:=Freeable); auto with mem.
+          apply J2.
+          simpl. clear.
+          assert (J:=@bytesize_chunk_pos 7).
+          zauto.
+
+          rewrite Int.signed_repr in J1; zauto. clear.
+          assert (J1:=@Int.min_signed_neg 31).          
+          assert (J2:=@Int.max_signed_pos 31).          
+          zauto.
+
+          assert (0 <= Size.to_Z tsz * n) as GE.
+            admit. (* tsz * n >= 0 *)
+          simpl. rewrite bytesize_chunk_7_eq_1. 
+          destruct J1 as [_ J1].
+          unfold Int.signed in J1.
+          unfold Int.unsigned in J1.
+          simpl in J1.
+          clear - J1 GE.
+          assert (J:=@Int.modulus_pos 31).
+          assert ((Size.to_Z tsz * n) mod Int.modulus 31 <= (Size.to_Z tsz * n)) 
+            as LE.
+            apply Zmod_le; zauto.
+          destruct (zlt ((Size.to_Z tsz * n) mod Int.modulus 31) 
+            (Int.half_modulus 31)); zeauto.
+
+          simpl. rewrite bytesize_chunk_7_eq_1. zauto.
+
+  SCase "id0<>i0".
+      rewrite <- lookupAL_updateAddAL_neq in J; auto.
+      assert (J':=@Hwfr i0 gvb gve J). clear Hwfr.    
+      eapply alloc_preserves_wf_data; eauto.
+Qed.
+
+Lemma malloc_preserves_wf_mmetadata : forall
+  (TD : TargetData)
+  (lc : GVMap)
+  (gl : GVMap)
+  (id0 : atom)
+  (t : typ)
+  (v : value)
+  (gn : GenericValue)
+  (align0 : align)
+  (Mem0 : mem)
+  (MM : mmetadata)
+  (als : list mblock)
+  (Mem' : mem)
+  (tsz : sz)
+  (mb : mblock)
+  (lc' : GVMap)
+  (rm' : rmetadata)
+  (n : Z) rm
+  (H : getTypeAllocSize TD t = ret tsz)
+  (H0 : getOperandValue TD Mem0 v lc gl = ret gn)
+  (H1 : malloc TD Mem0 tsz gn align0 = ret (Mem', mb))
+  (H2 : GV2int TD Size.ThirtyTwo gn = ret n)
+  (H3 : prop_reg_metadata lc rm id0 (blk2GV TD mb)
+         {| md_base := base2GV TD mb; md_bound := bound2GV TD mb tsz n |} =
+       (lc', rm'))
+  (Hwfm : wf_mmetadata TD Mem0 MM),
+  wf_mmetadata TD Mem' MM.
+Proof.
+  intros.
+  invert_prop_reg_metadata. clear H3.
+  unfold malloc in H1.
+  rewrite H2 in H1.
+  remember (Mem.alloc Mem0 0 (Size.to_Z tsz * n)) as R.
+  inversion H1. clear H1. subst.
+  intros b ofs gvb gve J.
+  assert (J':=@Hwfm b ofs gvb gve J). clear Hwfm.
+  eapply alloc_preserves_wf_data; eauto.
+Qed.
+
+Lemma free_preserves_wf_global_ptr : forall S TD Mem0 gl als Mem',
+  free TD Mem0 als = ret Mem' ->
+  wf_global_ptr S TD Mem0 gl ->
+  wf_global_ptr S TD Mem' gl.
+Admitted.
+
+Lemma free_allocas_preserves_wf_global_ptr : forall S TD Mem0 gl als Mem',
+  free_allocas TD Mem0 als = ret Mem' ->
+  wf_global_ptr S TD Mem0 gl ->
+  wf_global_ptr S TD Mem' gl.
+Admitted.
+
+Lemma malloc_preserves_wf_global_ptr : forall S TD Mem0 gl tsz gn align0 Mem' mb,
+  malloc TD Mem0 tsz gn align0 = ret (Mem', mb) ->
+  wf_global_ptr S TD Mem0 gl ->
+  wf_global_ptr S TD Mem' gl.
+Admitted.
+
+Lemma store_preserves_wf_global_ptr : forall S TD Mem0 gl gvp t gv align Mem',
+  mstore TD Mem0 gvp t gv align = Some Mem' ->
+  wf_global_ptr S TD Mem0 gl ->
+  wf_global_ptr S TD Mem' gl.
+Admitted.
+
+Lemma returnUpdateLocals__wf_rmetadata : forall los nts Result lc rm gl c' lc' 
+    rm' Mem0 Mem' als lc'' rm'' S Ps f rt
+  (Hwfg : wf_global_ptr S (los, nts) Mem0 gl)
+  (Hwfv : wf_value S (module_intro los nts Ps) f Result rt)
+  (H0 : free_allocas (los, nts) Mem0 als = ret Mem')
+  (H1 : returnUpdateLocals (los, nts) Mem' c' Result lc lc' rm rm' gl =
+       ret (lc'', rm''))
+  (Hwfm1' : wf_rmetadata (los, nts) Mem0 rm)
+  (Hwfm2' : wf_rmetadata (los, nts) Mem0 rm'),
+  wf_rmetadata (los, nts) Mem' rm''.
+Proof.
+  intros.
+  unfold returnUpdateLocals in H1.
+  assert (wf_rmetadata (los, nts) Mem' rm') as Hwfm.
+    eauto using free_allocas_preserves_wf_rmetadata.
+  destruct c'; try solve [inv H1; auto].
+  destruct n; try solve [inv H1; auto].
+  remember (getOperandValue (los, nts) Mem' Result lc gl) as R1.
+  destruct R1; try solve [inv H1; auto].
+  destruct t; try solve [inv H1; auto].
+  destruct t; try solve [inv H1; auto].
+  remember (get_reg_metadata (los, nts) Mem' gl rm Result) as R3.
+  destruct R3 as [[md ?]|]; inv H1; auto.
+    intros x gvb gve Hlk.
+    destruct (eq_atom_dec i0 x); subst.
+      rewrite lookupAL_updateAddAL_eq in Hlk.
+      inv Hlk. symmetry in HeqR3.
+      eapply wf_rmetadata__get_reg_metadata with (rm:=rm); eauto.
+        eapply free_allocas_preserves_wf_global_ptr in H0; eauto.
+        eapply free_allocas_preserves_wf_rmetadata in H0; eauto.
+
+      rewrite <- lookupAL_updateAddAL_neq in Hlk; eauto.
+
+    intros x gvb gve Hlk.
+    destruct (eq_atom_dec i0 x); subst.
+      rewrite lookupAL_updateAddAL_eq in Hlk.
+      inv Hlk. apply null_is_wf_data.
+
+      rewrite <- lookupAL_updateAddAL_neq in Hlk; eauto.
+Qed.
+
+Lemma updateValuesForNewBlock__wf_rmetadata : forall rvs TD M lc rm lc' rm',
+  wf_rmetadata TD M rm ->
+  updateValuesForNewBlock rvs lc rm = (lc', rm') ->
+  wf_rmetadata TD M rm'.
+Proof.
+  induction rvs; simpl; intros TD M lc rm lc' rm' Hwfr Hupdate.
+    inv Hupdate; auto.
+
+    destruct a. destruct p.
+    remember (updateValuesForNewBlock rvs lc rm) as R.
+    destruct R as [lc1 rm1].
+    destruct o as [[md ?]|]; inv Hupdate; eauto.
+Admitted.     
+      
+Lemma switchToNewBasicBlock__wf_rmetadata : forall TD M b1 b2 gl lc rm lc' rm',
+  wf_rmetadata TD M rm ->
+  switchToNewBasicBlock TD M b1 b2 gl lc rm = Some (lc', rm') ->
+  wf_rmetadata TD M rm'.
+Proof.
+  intros TD M b1 b2 gl lc rm lc' rm' Hwfr Hswitch.
+  unfold switchToNewBasicBlock in Hswitch.
+  remember (getIncomingValuesForBlockFromPHINodes TD M 
+             (getPHINodesFromBlock b1) b2 gl lc rm) as R.
+  destruct R; inv Hswitch.
+  eapply updateValuesForNewBlock__wf_rmetadata; eauto.
+Qed.
+
+Lemma get_mem_metadata__wf_rmetadata : forall los nts Mem0 rm gvp id0 MM,
+  wf_mmetadata (los, nts) Mem0 MM ->
+  wf_rmetadata (los, nts) Mem0 rm ->
+  wf_rmetadata (los, nts) Mem0 
+    (updateAddAL metadata rm id0 (get_mem_metadata (los, nts) MM gvp)).
+Proof.
+  intros.
+  intros i0 gvb gve J.
+  destruct (@id_dec id0 i0); subst.
+    rewrite lookupAL_updateAddAL_eq in J.
+    inversion J; subst.
+    eapply wf_mmetadata__get_mem_metadata in H2; eauto.
+
+    rewrite <- lookupAL_updateAddAL_neq in J; auto. eauto.
+Qed.
+
+
+Lemma store_preserves_wf_rmetadata : forall TD Mem0 gvp t gv align0 Mem' rm, 
+  mstore TD Mem0 gvp t gv align0 = ret Mem' ->
+  wf_rmetadata TD Mem0 rm -> 
+  wf_rmetadata TD Mem' rm.
+Proof. 
+  intros TD Mem0 gvp t gv align0 Mem' rm H3 Hwfr.
+  unfold mstore in H3.
+  destruct (GV2ptr TD (getPointerSize TD) gvp); try solve [inversion H3].
+  destruct v; try solve [inversion H3].
+  destruct (typ2memory_chunk t); try solve [inversion H3].
+  destruct (GV2val TD gv); try solve [inversion H3].
+  intros i1 gvb gve J.
+  apply Hwfr in J. clear Hwfr.
+  eapply wf_data__store__wf_data; eauto.
+Qed.
+
+Lemma store_nptr_preserves_wf_mmetadata : forall TD Mem0 gvp t gv align0 Mem' MM,
+  mstore TD Mem0 gvp t gv align0 = ret Mem' ->
+  wf_mmetadata TD Mem0 MM -> 
+  wf_mmetadata TD Mem' MM.
+Proof. 
+  intros TD Mem0 gvp t gv align0 Mem' rm H3 Hwfm.
+  unfold mstore in H3.
+  destruct (GV2ptr TD (getPointerSize TD) gvp); try solve [inversion H3].
+  destruct v; try solve [inversion H3].
+  destruct (typ2memory_chunk t); try solve [inversion H3].
+  destruct (GV2val TD gv); try solve [inversion H3].
+  intros b0 ofs gvb gve J.
+  apply Hwfm in J. clear Hwfm.
+  eapply wf_data__store__wf_data; eauto.
+Qed.
+
+Lemma store_ptr_preserves_wf_mmetadata : forall los nts Mem0 rm MM md' mt' gl S
+    gvp gv align0 Mem' Ps f v t
+  (Hwfg' : wf_global_ptr S (los, nts) Mem0 gl)
+  (Hwfm1' : wf_rmetadata (los, nts) Mem0 rm)
+  (H3 : mstore (los, nts) Mem0 gvp t gv align0 = ret Mem')
+  (H5 : get_reg_metadata (los, nts) Mem0 gl rm v = ret (md', mt'))
+  (Hwfv : wf_value S (module_intro los nts Ps) f v t)
+  (Hwfm : wf_mmetadata (los, nts) Mem0 MM),
+  wf_mmetadata (los, nts) Mem' (set_mem_metadata (los, nts) MM gvp md').
+Proof.
+  intros.
+  unfold mstore in H3.
+  destruct (GV2ptr (los,nts) (getPointerSize (los,nts)) gvp); 
+    try solve [inversion H3].
+  destruct v0; try solve [inversion H3].
+  destruct (typ2memory_chunk t); try solve [inversion H3].
+  destruct (GV2val (los,nts) gv); try solve [inversion H3].
+  intros b0 ofs gvb gve J. 
+    subst.
+    unfold set_mem_metadata in J.
+    destruct (GV2ptr (los,nts) (getPointerSize (los,nts)) gvp); 
+      try solve [eauto using wf_mmetadata__store__wf_data].
+    destruct v1; try solve [eauto using wf_mmetadata__store__wf_data].
+    destruct (zeq b0 b1); subst; 
+       simpl in J; eauto using wf_mmetadata__store__wf_data.
+    destruct (Int.eq_dec 31 i1 ofs); subst; 
+       simpl in J; eauto using wf_mmetadata__store__wf_data.
+  
+       inversion J; subst. clear J.
+       eapply wf_rmetadata__get_reg_metadata in H5; eauto.
+         eapply wf_data__store__wf_data; eauto.
+Qed.
+
+Lemma prop_metadata_preserves_wf_rmetadata : forall los nts Mem0 rm md mt gl S Ps
+    f t id0 vp
+  (H : get_reg_metadata (los, nts) Mem0 gl rm vp = ret (md, mt))
+  (Hwfg' : wf_global_ptr S (los, nts) Mem0 gl)
+  (Hwfv : wf_value S (module_intro los nts Ps) f vp t)
+  (Hwfr : wf_rmetadata (los, nts) Mem0 rm),
+  wf_rmetadata (los, nts) Mem0 (updateAddAL metadata rm id0 md).
+Proof.
+  intros.
+  intros i0 gvb gve J0.
+  destruct (@id_dec id0 i0); subst.
+    rewrite lookupAL_updateAddAL_eq in J0.
+    inversion J0; subst. clear J0.
+    eapply wf_rmetadata__get_reg_metadata in H; eauto.
+
+    rewrite <- lookupAL_updateAddAL_neq in J0; auto.
+    apply Hwfr in J0; auto.
+Qed.
+
+Lemma initLocals__wf_rmetadata : forall ogvs (rm : rmetadata) (lc' : GVMap) 
+  Mem0 rm' TD la, 
+  initLocals la ogvs rm = (lc', rm') ->
+  wf_rmetadata TD Mem0 rm'.
+Admitted.
+
+Lemma callExternalFunction_preserves_wf_rmetadata : forall Mem0 fid gvs oresult
+    Mem' rm TD,
+  callExternalFunction Mem0 fid gvs = (oresult, Mem') ->
+  wf_rmetadata TD Mem0 rm ->
+  wf_rmetadata TD Mem' rm.
+Admitted.
+
+Lemma callExternalFunction_preserves_wf_mmetadata : forall Mem0 fid gvs oresult
+    Mem' TD MM,
+  callExternalFunction Mem0 fid gvs = (oresult, Mem') ->
+  wf_mmetadata TD Mem0 MM ->
+  wf_mmetadata TD Mem' MM.
+Admitted.
+
+Lemma callExternalFunction_preserves_wf_global_ptr : forall Mem0 fid gvs oresult
+    Mem' S TD gl,
+  callExternalFunction Mem0 fid gvs = (oresult, Mem') ->
+  wf_global_ptr S TD Mem0 gl ->
+  wf_global_ptr S TD Mem' gl.
+Admitted.
+
+Lemma adding_null_preserves_wf_rmetadata : forall TD Mem0 rm id0,
+  wf_rmetadata TD Mem0 rm ->
+  wf_rmetadata TD Mem0
+    (updateAddAL metadata rm id0 {| md_base := null; md_bound := null |}).
+Proof.
+  intros TD Mem0 rm id0 Hwfr.
+  intros i0 gvb gve J.
+  destruct (@id_dec id0 i0); subst.
+    rewrite lookupAL_updateAddAL_eq in J.
+    inversion J; subst. clear J.
+    unfold wf_data.
+    simpl.
+    split.
+      apply nullptr_lt_nextblock.
+  
+      intros Htmp ofs J.
+      contradict J; zauto.
+  
+    rewrite <- lookupAL_updateAddAL_neq in J; auto.
+    apply Hwfr in J; auto.
+Qed.
+
+
+(*****************************)
+(*
+*** Local Variables: ***
+*** coq-prog-name: "coqtop" ***
+*** coq-prog-args: ("-emacs-U" "-I" "~/SVN/sol/vol/src/ssa/monads" "-I" "~/SVN/sol/vol/src/ssa/ott" "-I" "~/SVN/sol/vol/src/ssa/compcert" "-I" "~/SVN/sol/theory/metatheory_8.3" "-I" "~/SVN/sol/vol/src/TV") ***
+*** End: ***
+ *)
